Progress on the new version. Only 2 non-trivial admits to go.

newio/DM6.fst
@@ -92,131 +92,6 @@ let dm_subcomp (a:Type) (wp1 wp2: hist a) (f : dm a wp1) :
 let dm_if_then_else (a : Type) (wp1 wp2: hist a) (f : dm a wp1) (g : dm a wp2) (b : bool) : Type =
   dm a (hist_if_then_else wp1 wp2 b)
 
-////////////////////////////////////////////////////////////////////////////////////////
-
-let io_subcomp (a:Type)
-  (q1:pure_post a) (q2:pure_post a)
-  (m : io (v:a{q1 v})) :
-  Pure (io (v:a{q2 v})) 
-    (requires (forall x. q1 x ==> q2 x))
-    (ensures (fun r -> True)) =
-  admit ();
-  m
-
-unfold
-let pure_post_return (x:'a) : pure_post 'a = fun y -> x == y
-
-unfold
-let pure_post_bind (#a #b:Type) (q1:pure_post a) (q2:a -> pure_post b) : pure_post b =
-  fun y -> exists (x:a{q1 x}). q2 x y
-
-unfold
-let pure_post_if_then_else (q1 q2:pure_post 'a) (b:bool) : pure_post 'a =
-  fun x -> (b ==> q1 x) /\ ((~b) ==> q2 x)
-
-/////////////////////////////////////////////////////////////////////////////////////
-
-(** Later we refine the output type of the dijkstra monad with the pure post condition (q),
-which forces us to index the dijkstra monad by a weakest-precondition of type `hist (v:a{q v})`.
-For cleanliness reasons, we define a synonym for that called `histq`. **)
-
-unfold
-let histq #event a (q:pure_post a) = hist #event (v:a{q v})
-
-unfold
-let histq_ord
-  (#q1:pure_post 'a) (#q2:pure_post 'a)
-  (wp1: histq 'a q1) 
-  (wp2: histq 'a q2) :
-  Pure Type0
-    (requires (forall x. q2 x ==> q1 x))
-    (ensures (fun _ -> True)) =
-  forall h (p:hist_post (v:'a{q1 v})). 
-    wp1 p h ==> wp2 (fun lt (r:'a{q2 r}) -> p lt (r <: (x:'a{q1 x}))) h
-
-unfold
-let histq_return (x:'a) : histq 'a (pure_post_return x) =
-  hist_return x
-
-let lemma_histq_subcomp_post
-  (a b:Type)
-  (q1:pure_post a) (q2:a -> pure_post b)
-  (wp:(x:a{q1 x}) -> histq b (q2 x)) 
-  (x: a{q1 x})
-  (p1 p2 : hist_post (v:b{pure_post_bind q1 q2 v}))
-  (h:trace) :
-  Lemma
-    (requires (p1 `hist_post_ord` p2 /\ wp x (fun lt r -> p1 lt r) h))
-    (ensures (wp x (fun lt r -> p2 lt r) h)) = ()
-
-unfold
-let histq_subcomp_bind
-  (a b:Type)
-  (q1:pure_post a) (q2:a -> pure_post b)
-  (wp2:(x:a) -> histq b (q2 x)) 
-  (x: a{q1 x}) :
-  Tot (histq b (pure_post_bind q1 q2)) = 
-  Classical.forall_intro_3 (Classical.move_requires_3 (lemma_histq_subcomp_post a b q1 q2 wp2 x));
-  fun p -> wp2 x (fun lt (r: b{q2 x r}) -> p lt r)
-
-unfold
-let histq_if_then_else (q1 q2:pure_post 'a) (wp1:histq 'a q1) (wp2:histq 'a q2) (b:bool) : histq 'a (pure_post_if_then_else q1 q2 b) by (
-  explode ()
-)=
-  admit ();
-  (** TODO: show that histq_if_then_else is monotonic **)
-  fun (p:trace -> (x:'a{pure_post_if_then_else q1 q2 b x}) -> Type0) h -> (b ==> wp1 p h) /\ ((~b) ==> wp2 p h)
-
-let dm_subcomp_histq (a:Type) 
-  (q1:pure_post a) (q2:pure_post a)
-  (wp1: histq a q1) 
-  (wp2: histq a q2)
-  (f : dm (v:a{q1 v}) wp1) :
-  Pure (dm (v:a{q2 v}) wp2)
-    (requires ((forall x. q1 x ==> q2 x) /\ wp2 `histq_ord` wp1))
-    (ensures fun _ -> True) =
-  assert (wp1 `hist_ord` (theta f));
-  assert (wp2 `histq_ord` wp1);
-
-  let m = io_subcomp a q1 q2 f in
-  assert (wp2 `hist_ord` (theta m));
-  m
-
-/////////////////////////////////////////////////////////////////////////////
-
-let dmq (a:Type) (q:pure_post a) (wp:histq a q) = 
-  dm (v:a{q v}) wp 
-
-let dmq_return (a:Type) (x:a) : dmq a (pure_post_return x) (histq_return x) = 
-  dm_return _ x
-
-let dmq_bind (a b:Type)
-  (q1:pure_post a) (q2:a -> pure_post b)
-  (wp1:histq a q1) (wp2:(x:a) -> histq b (q2 x))
-  (f:dmq a q1 wp1) 
-  (g:(x:a{q1 x}) -> dmq b (q2 x) (wp2 x)) :
-  Tot (dmq b (pure_post_bind q1 q2) (hist_bind wp1 (histq_subcomp_bind a b q1 q2 wp2))) =
-    dm_bind 
-      (v:a{q1 v})
-      (v:b{pure_post_bind q1 q2 v})
-      wp1
-      (histq_subcomp_bind a b q1 q2 wp2)
-      f
-      (fun (x:a{q1 x}) -> 
-        dm_subcomp_histq b
-         (q2 x) (pure_post_bind q1 q2)
-         (wp2 x)
-         (histq_subcomp_bind a b q1 q2 wp2 x)
-         (g x))
-
-let dmq_subcomp (a:Type) (q1 q2:pure_post a) (wp1:hist (v:a{q1 v})) (wp2:hist (v:a{q2 v})) (f:dmq a q1 wp1) :
-  Pure (dmq a q2 wp2)
-    (requires (
-      (forall x. q1 x ==> q2 x) /\
-      (wp2 `histq_ord` wp1)))
-    (ensures fun _ -> True) =
-  dm_subcomp_histq a q1 q2 wp1 wp2 f
-
 ///////////////////////////////////////////////////////////////////////////
 
 let hist_as_requires (wp:hist 'a) = forall h. wp (fun _ _ -> True) h
@@ -227,18 +102,32 @@ let pdmq (a:Type) (wp:hist a) =
 let pdmq_return (a:Type) (x:a) : pdmq a (hist_return x) =
   fun _ -> dm_return _ x
 
-let pdmq_bind (a b:Type)
+unfold
+let hist_bind_v2 (wp1 : hist 'a) (wp2 : 'a -> hist 'b) : hist 'b =
+  fun p2 h -> (forall (p1:hist_post 'a). wp1 p1 h /\ (forall (lt:trace) r. p1 lt r ==> (wp2 r p2 (List.rev lt @ h))))
+
+let lemma_hist_bind_implies_hist_bind_v2 (w : hist 'a) (kw : 'a -> hist 'b) :
+  Lemma (hist_bind w kw `hist_ord` hist_bind_v2 w kw) = admit ()
+  
+let pdmq_bind_v2_0 (a b:Type)
   (wp1:hist a) (wp2:(x:a) -> hist b)
   (f:pdmq a wp1) 
   (g:(x:a) -> pdmq b (wp2 x))
-  (pre:squash (forall r l p h. wp1 p h /\ (p l r ==> (hist_as_requires (wp2 r))))) :
-  Tot (dm b (hist_bind wp1 wp2)) =
-  assume (hist_as_requires wp1); (** this should be easy to prove by instantiating pre **)
+  (pre:squash (hist_as_requires (hist_bind_v2 wp1 wp2))) :
+  Tot (dm b (hist_bind_v2 wp1 wp2)) =
+  assert (hist_as_requires wp1); (** this should be easy to prove by instantiating pre **)
   dm_bind a b wp1 wp2 (f _) (fun (x:a) -> 
-    assert (forall l p h. wp1 p h /\ (p l x ==> (hist_as_requires (wp2 x))));
-    assume (exists l. forall p h. wp1 p h /\ p l x);
+    (** the f returned an x, therefore it exists a lt s.t. the following prop should be valid **)
+    assume (exists lt. forall p1 h. wp1 p1 h /\ p1 lt x);
     assert (hist_as_requires (wp2 x));
     g x _)
+
+let pdmq_bind_v2 (a b:Type)
+  (wp1:hist a) (wp2:(x:a) -> hist b)
+  (f:pdmq a wp1) 
+  (g:(x:a) -> pdmq b (wp2 x)) :
+  pdmq b (hist_bind_v2 wp1 wp2) =
+  pdmq_bind_v2_0 a b wp1 wp2 f g 
 
 let pdmq_subcomp (a:Type) (wp1:hist a) (wp2:hist a) (f:pdmq a wp1) :
   Pure (pdmq a wp2)
@@ -246,6 +135,16 @@ let pdmq_subcomp (a:Type) (wp1:hist a) (wp2:hist a) (f:pdmq a wp1) :
       (wp2 `hist_ord` wp1)))
     (ensures fun _ -> True) =
   fun _ -> dm_subcomp a wp1 wp2 (f ())
+  
+let pdmq_bind (a b:Type)
+  (wp1:hist a) (wp2:(x:a) -> hist b)
+  (f:pdmq a wp1) 
+  (g:(x:a) -> pdmq b (wp2 x)) :
+  pdmq b (hist_bind wp1 wp2) =
+  lemma_hist_bind_implies_hist_bind_v2 wp1 wp2;
+  assert ((hist_bind wp1 wp2) `hist_ord` (hist_bind_v2 wp1 wp2)); 
+  pdmq_subcomp _ (hist_bind_v2 wp1 wp2) (hist_bind wp1 wp2) (pdmq_bind_v2 a b wp1 wp2 f g) 
+
   
 unfold
 let pdmq_if_then_else 
@@ -277,39 +176,25 @@ effect IO
   (pre : trace -> Type0)
   (post : trace -> trace -> a -> Type0) =
   IOwp a 
-    (fun _ -> True)
     (fun (p:hist_post a) (h:trace) -> pre h /\ (forall lt r. post h lt r ==>  p lt r)) 
 
-
-unfold let as_requires (#a: Type) (wp: pure_wp a) = wp (fun x -> True)
-unfold let as_ensures (#a: Type) (wp: pure_wp a) (x: a) = ~(wp (fun y -> (y =!= x)))
-
-unfold
-let histq_for_pure (#event #a:Type) (pre:pure_pre) q : histq #event a q = fun p h -> pre /\ (forall (r:a{q r}). p [] r)
-
-(** histq_for_pure is labeled with unfold, but when trying to prove the lift,
-the unfolding confuses
-the SMT. Therefore, the following is just a trick to get an automated proof of the lift **)
-let histq_for_pure0 (#event #a:Type) = histq_for_pure #event #a
 let lift_pure_pdmq0 (a : Type) (w : pure_wp a) (f:(eqtype_as_type unit -> PURE a w)) :
-  pdmq a (as_ensures w) (histq_for_pure0 (as_requires w) (as_ensures w)) =
-  fun (pre:squash (forall h. histq_for_pure0 #event #a (as_requires w) (as_ensures w) (fun _ _ -> True) h)) ->
-    assert (forall h. histq_for_pure0 #event #a (as_requires w) (as_ensures w) (fun _ _ -> True) h); 
-    assert ((forall h. histq_for_pure0 #event #a (as_requires w) (as_ensures w) (fun _ _ -> True) h) ==>
+  pdmq a (wp_lift_pure_hist w) =
+  fun (pre:squash (hist_as_requires (wp_lift_pure_hist w))) ->
+    assert (hist_as_requires (wp_lift_pure_hist #a w) ==>
         as_requires w) by (
-        norm [delta_only [`%histq_for_pure0;`%histq_for_pure]];
+        norm [delta_only [`%wp_lift_pure_hist; `%hist_as_requires;`%as_requires]];
         let impl = implies_intro () in
         let impl = instantiate impl (`([])) in
-        let lhs, _ = destruct_and impl in
         assumption ()
     );
     FStar.Monotonic.Pure.elim_pure_wp_monotonicity_forall ();
     let r = f () in
-    let r' = dmq_return _ r in
-    dmq_subcomp _ _ _ _ _ r'
+    let r' = dm_return _ r in
+    dm_subcomp _ _ _ r'
 
 let lift_pure_pdmq (a : Type) (w : pure_wp a) (f:(eqtype_as_type unit -> PURE a w)) :
-  pdmq a (as_ensures w) (histq_for_pure (as_requires w) (as_ensures w)) =
+  pdmq a (wp_lift_pure_hist w) =
     lift_pure_pdmq0 a w f
 
 sub_effect PURE ~> IOwp = lift_pure_pdmq
